start on compile_decs_thm
but want to remove the optimisation for a single dec - the proof is more
uniform if the implementation unwraps the tuple, then immediately
re-wraps it to pop the exception, then unwraps it again. (in the general
case the wrap is of more stuff than just the tuple that was just
unwrapped.)

could prove as a bytecode optimisation that an unwrap followed by a wrap
is a no-op, then compile_decs wouldn't have to special-case. (or could
then define the optimised compile_decs and show it produces equivalent
bytecode.)

compiler/proofs/compilerProofsScript.sml
@@ -1958,6 +1958,154 @@ val FV_decs_def = Define`
 
 ---8<---
 
+  compile_decs_def
+  compile_dec_append_out
+
+val decs_cns_def = Define`
+  (decs_cns _ [] = {}) ∧
+  (decs_cns mn (d::ds) = dec_cns d ∪ (decs_cns mn ds DIFF (IMAGE (mk_id mn) (set (new_dec_cns d)))))`
+
+val evaluate_dec_err_cenv_emp = store_thm("evaluate_dec_err_cenv_emp",
+  ``∀mn menv cenv s env d res. evaluate_dec mn menv cenv s env d res ⇒
+    ∀err. SND res = Rerr err ∧ err ≠ Rtype_error ⇒ dec_to_cenv mn d = []``,
+  ho_match_mp_tac evaluate_dec_ind >> simp[dec_to_cenv_def])
+
+val evaluate_dec_new_dec_cns = store_thm("evaluate_dec_new_dec_cns",
+  ``∀mn menv cenv s env d res. evaluate_dec mn menv cenv s env d res ⇒
+    ∀tds env. SND res = Rval (tds,env) ⇒
+    MAP (mk_id mn) (new_dec_cns d) = (MAP FST tds)``,
+  ho_match_mp_tac evaluate_dec_ind >>
+  simp[LibTheory.emp_def,SemanticPrimitivesTheory.build_tdefs_def] >>
+  rw[] >>
+  simp[MAP_MAP_o,MAP_FLAT] >> AP_TERM_TAC >>
+  simp[MAP_EQ_f,FORALL_PROD,MAP_MAP_o])
+
+val evaluate_dec_dec_to_cenv = store_thm("evaluate_dec_dec_to_cenv",
+  ``∀mn menv cenv s env d res. evaluate_dec mn menv cenv s env d res ⇒
+    ∀tds env. SND res = Rval (tds,env) ⇒
+    tds = dec_to_cenv mn d``,
+  ho_match_mp_tac evaluate_dec_ind >>
+  simp[LibTheory.emp_def,dec_to_cenv_def])
+
+val compile_decs_thm = store_thm("compile_decs_thm",
+  ``∀mn menv cenv s env decs res.
+    evaluate_decs mn menv cenv s env decs res ⇒
+    ∃ck. ∀rmenv ct m renv rsz cs ct' m' rsz' cs' code cenv0 env0 rs0 rs rd bs bc0 ig h0 sp st0.
+    compile_decs mn rmenv ct m renv rsz cs decs = (ct',m',rsz',cs')
+    ∧ cs'.out = REVERSE code ++ cs.out
+    ∧ closed_context menv cenv s env
+    ∧ FV_decs decs ⊆ set (MAP (Short o FST) env) ∪ menv_dom menv
+    ∧ "" ∉ new_decs_cns decs
+    ∧ decs_cns mn decs ⊆ set (MAP FST cenv)
+    ∧ env_rs menv cenv0 env0 rs0 (LENGTH st0) rd (ck,s) (bs with <|code := bc0; stack := st0|>)
+    ∧ env_rs menv cenv env rs (LENGTH st0) rd (ck,s) (bs with code := bc0)
+    ∧ rs.rsz = rsz
+    ∧ rs.rnext_label = cs.next_label
+    ∧ rs.contab = ct
+    ∧ bs.code = bc0 ++ code
+    ∧ bs.pc = next_addr bs.inst_length bc0
+    ∧ bs.stack = ig ++ StackPtr h0::CodePtr sp::st0
+    ∧ bs.handler = LENGTH st0 + 1
+    ∧ IS_SOME bs.clock
+    ∧ good_labels rs.rnext_label bc0
+    ⇒
+    case SND(SND res) of
+    | Rval env' =>
+      ∃bvs rf rd'.
+      let s' = FST res in
+      let bs' = bs with <|pc := next_addr bs.inst_length (bc0 ++ code); stack := bvs++bs.stack; refs := rf; clock := SOME 0|> in
+      let n = rsz' - rsz in
+      let rs' = rs with <|rnext_label := cs'.next_label
+                         ;contab := ct'
+                         ;renv := ZIP(TAKE n m'.bvars,GENLIST (λi. rsz+i) n) ++ rs.renv
+                         ;rsz := rsz'
+                         |> in
+      bc_next^* bs bs'
+      ∧ env_rs menv (FST(SND res)++cenv) (env'++env) rs' (LENGTH st0) rd' (0,s') bs'
+      ∧ env_rs menv cenv0 env0 rs0 (LENGTH st0) rd' (0,s') (bs' with stack := st0)
+    | Rerr(Rraise err) =>
+      ∃bv rf rd'.
+      let s' = FST res in
+      let bs' = bs with <|pc := sp; stack := bv::st0; handler := h0; refs := rf; clock := SOME 0|> in
+      let rs0' = rs0 with contab := decs_to_contab mn rs0.contab decs in
+      bc_next^* bs bs'
+      ∧ err_bv err bv
+      ∧ env_rs menv (FST(SND res)++cenv0) env0 rs0' (LENGTH st0) rd' (0,s') (bs' with stack := st0)
+    | _ => T``,
+  ho_match_mp_tac evaluate_decs_ind >>
+  strip_tac >- (
+    simp[compile_decs_def] >>
+    simp[decs_cns_def,FV_decs_def,Once SWAP_REVERSE,LibTheory.emp_def] >>
+    rpt gen_tac >>
+    qexists_tac`0` >>
+    rpt gen_tac >>
+    strip_tac >>
+    map_every qexists_tac [`[]`,`bs.refs`,`rd`] >>
+    simp[] >>
+    `bs.clock = SOME 0` by (
+      Cases_on`bs.clock`>>fs[env_rs_def,LET_THM,Cenv_bs_def,s_refs_def] ) >>
+    conj_tac >- (
+      simp[Once RTC_CASES1] >>
+      disj1_tac >>
+      simp[bc_state_component_equality] ) >>
+    conj_tac >- (
+      qmatch_abbrev_tac`env_rs menv cenv env rs' rsz rd cks bs'` >>
+      `rs' = rs ∧ bs' = bs` by (
+        simp[Abbr`rs'`,Abbr`bs'`,bc_state_component_equality,compiler_state_component_equality] ) >>
+      simp[] ) >>
+    qmatch_abbrev_tac`env_rs menv cenv0 env0 rs0 rsz rd cks bs'` >>
+    `bs' = bs with stack := st0` by (
+      simp[Abbr`bs'`,bc_state_component_equality] ) >>
+    simp[] ) >>
+  strip_tac >- (
+    simp[compile_decs_def] >>
+    rpt gen_tac >> strip_tac >>
+    imp_res_tac compile_dec_thm >>
+    qexists_tac`ck` >>
+    rpt gen_tac >>
+    qabbrev_tac`p = compile_dec rmenv m renv rs.rsz cs d` >>
+    PairCases_on`p`>>fs[]>>
+    Cases_on`e = Rtype_error`>>simp[]>>
+    `∃vs. p0 = SOME vs` by (
+      Cases_on`d`>>fs[compile_dec_def,LET_THM,markerTheory.Abbrev_def]>>
+      last_x_assum mp_tac >>
+      simp[Once evaluate_dec_cases] ) >>
+    simp[]
+
+      match_mp_tac R
+
+    compile_decs_def
+
+  ``∀mno menv cenv s env dec res. evaluate_decs mno menv cenv s env dec res ⇒
+     ∀mn rs. ∃ck. ∀rs' bc00 rd bc bs bc0.
+      (mno = SOME mn) ∧
+      closed_context menv cenv s env ∧
+      FV_decs dec ⊆ set (MAP (Short o FST) env) ∪ menv_dom menv ∧
+      ("" ∉ new_decs_cns dec) ∧
+      decs_cns mn dec ⊆ set (MAP FST cenv) ∧
+      (∀i tds. i < LENGTH dec ∧ (EL i dec = Dtype tds) ⇒ check_dup_ctors mno (decs_to_cenv mno (TAKE i dec) ++ cenv) tds) ∧
+      env_rs menv cenv env rs rd (ck,s) (bs with code := bc0) ∧
+      (compile_decs mn dec (rs,bc00) = (rs',(REVERSE bc)++bc00)) ∧
+      (bs.code = bc0 ++ bc) ∧
+      (bs.pc = next_addr bs.inst_length bc0) ∧
+      IS_SOME bs.clock ∧
+      good_labels rs.rnext_label bc0
+      ⇒
+      case res of (s',cenv',Rval(env')) =>
+        ∃st rf rd'.
+        let bs' = bs with <|pc := next_addr bs.inst_length (bc0 ++ bc); stack := st; refs := rf; clock := SOME 0|> in
+        bc_next^* bs bs' ∧
+        env_rs menv (cenv'++cenv) (env'++env) rs' rd' (0,s') bs'
+      | (s',_emp,Rerr(Rraise err)) =>
+        ∃bv rf rd'.
+        let cenv' = decs_to_cenv mno dec in
+        let bs' = bs with <|pc := 0; stack := bv::bs.stack; refs := rf; clock := SOME 0|> in
+        bc_next^*bs bs' ∧
+        err_bv err bv ∧
+        env_rs menv (cenv'++cenv) env (rs with contab := decs_to_contab mno rs.contab dec) rd' (0,s') (bs' with stack := bs.stack)
+      | (s',_) => T``,
+  ho_match_mp_tac evaluate_decs_strongind >>
+
 val compile_decs_append_out = store_thm("compile_decs_append_out",
   ``∀decs mn menv ct m env rsz cs.
     let (ct',m',rsz',cs') = compile_decs mn menv ct m env rsz cs decs in
@@ -1990,45 +2138,6 @@ val compile_decs_append_out = store_thm("compile_decs_append_out",
     simp[Once SWAP_REVERSE] >> rw[] >> fs[] >>
     fs[between_labels_def] ) >>
   Cases_on`mn`>>rw[]>>fs[]
-
-  compile_decs_def
-  compile_dec_append_out
-
-val compile_decs_thm = store_thm("compile_decs_thm",
-  ``∀mn menv cenv s env decs res.
-    evaluate_decs mn menv cenv s env decs res ⇒
-    ∃ck. ∀rmenv ct 
-    compile_decs_def
-
-  ``∀mno menv cenv s env dec res. evaluate_decs mno menv cenv s env dec res ⇒
-     ∀mn rs. ∃ck. ∀rs' bc00 rd bc bs bc0.
-      (mno = SOME mn) ∧
-      closed_context menv cenv s env ∧
-      FV_decs dec ⊆ set (MAP (Short o FST) env) ∪ menv_dom menv ∧
-      ("" ∉ new_decs_cns dec) ∧
-      decs_cns mn dec ⊆ set (MAP FST cenv) ∧
-      (∀i tds. i < LENGTH dec ∧ (EL i dec = Dtype tds) ⇒ check_dup_ctors mno (decs_to_cenv mno (TAKE i dec) ++ cenv) tds) ∧
-      env_rs menv cenv env rs rd (ck,s) (bs with code := bc0) ∧
-      (compile_decs mn dec (rs,bc00) = (rs',(REVERSE bc)++bc00)) ∧
-      (bs.code = bc0 ++ bc) ∧
-      (bs.pc = next_addr bs.inst_length bc0) ∧
-      IS_SOME bs.clock ∧
-      good_labels rs.rnext_label bc0
-      ⇒
-      case res of (s',cenv',Rval(env')) =>
-        ∃st rf rd'.
-        let bs' = bs with <|pc := next_addr bs.inst_length (bc0 ++ bc); stack := st; refs := rf; clock := SOME 0|> in
-        bc_next^* bs bs' ∧
-        env_rs menv (cenv'++cenv) (env'++env) rs' rd' (0,s') bs'
-      | (s',_emp,Rerr(Rraise err)) =>
-        ∃bv rf rd'.
-        let cenv' = decs_to_cenv mno dec in
-        let bs' = bs with <|pc := 0; stack := bv::bs.stack; refs := rf; clock := SOME 0|> in
-        bc_next^*bs bs' ∧
-        err_bv err bv ∧
-        env_rs menv (cenv'++cenv) env (rs with contab := decs_to_contab mno rs.contab dec) rd' (0,s') (bs' with stack := bs.stack)
-      | (s',_) => T``,
-  ho_match_mp_tac evaluate_decs_strongind >>
 
 val compile_dec_contab_thm = store_thm("compile_dec_contab_thm",
   ``∀mn rs dec menv cenv env rd cs bs cenv' rs'.
@@ -2425,10 +2534,6 @@ val FV_top_def = Define`
   (FV_top (Tmod mn _ ds) = FV_decs ds)`
 val _ = export_rewrites["FV_top_def"]
 
-val decs_cns_def = Define`
-  (decs_cns _ [] = {}) ∧
-  (decs_cns mn (d::ds) = dec_cns d ∪ (decs_cns mn ds DIFF (IMAGE (Long mn) (set (new_dec_cns d)))))`
-
 val top_cns_def = Define`
   (top_cns (Tdec d) = dec_cns d) ∧
   (top_cns (Tmod mn _ ds) = decs_cns mn ds)`
@@ -2526,11 +2631,6 @@ val env_rs_with_irr = store_thm("env_rs_with_irr",
     ⇒
     env_rs menv cenv env rs' rd cs bs``,
   simp[env_rs_def])
-
-val evaluate_dec_err_cenv_emp = store_thm("evaluate_dec_err_cenv_emp",
-  ``∀mn menv cenv s env d res. evaluate_dec mn menv cenv s env d res ⇒
-    ∀err. SND res = Rerr err ∧ err ≠ Rtype_error ⇒ dec_to_cenv mn d = []``,
-  ho_match_mp_tac evaluate_dec_ind >> simp[dec_to_cenv_def])
 
 (*
 val compile_fake_exp_val = store_thm("compile_fake_exp_val",
@@ -3309,23 +3409,6 @@ val evaluate_dec_closed_context = store_thm("evaluate_dec_closed_context",
       fsrw_tac[DNF_ss][MEM_MAP,SUBSET_DEF] >>
       metis_tac[] ) >>
     metis_tac[] ))
-
-val evaluate_dec_new_dec_cns = store_thm("evaluate_dec_new_dec_cns",
-  ``∀mn menv cenv s env d res. evaluate_dec mn menv cenv s env d res ⇒
-    ∀tds env. SND res = Rval (tds,env) ⇒
-    MAP (mk_id mn) (new_dec_cns d) = (MAP FST tds)``,
-  ho_match_mp_tac evaluate_dec_ind >>
-  simp[LibTheory.emp_def,SemanticPrimitivesTheory.build_tdefs_def] >>
-  rw[] >>
-  simp[MAP_MAP_o,MAP_FLAT] >> AP_TERM_TAC >>
-  simp[MAP_EQ_f,FORALL_PROD,MAP_MAP_o])
-
-val evaluate_dec_dec_to_cenv = store_thm("evaluate_dec_dec_to_cenv",
-  ``∀mn menv cenv s env d res. evaluate_dec mn menv cenv s env d res ⇒
-    ∀tds env. SND res = Rval (tds,env) ⇒
-    tds = dec_to_cenv mn d``,
-  ho_match_mp_tac evaluate_dec_ind >>
-  simp[LibTheory.emp_def,dec_to_cenv_def])
 
 val env_rs_change_clock = store_thm("env_rs_change_clock",
   ``∀menv cenv env rs rd cs bs cs' ck' bs'.
